---
source_image: page_163.png
page_number: 163
model: model-run-olm-ocr
prompt_type: olmocr_technical
processing_time: 30.52
tokens: 5741
characters: 2442
timestamp: 2025-12-24T07:09:04.621780
finish_reason: stop
---

998.
\[
\begin{pmatrix}
3\lambda^2 - 5\lambda + 2 & 0 & 3\lambda^2 - 6\lambda + 3 \\
2\lambda^2 - 3\lambda + 1 & \lambda - 1 & 2\lambda^2 - 4\lambda + 2 \\
2\lambda^2 - 2\lambda & 0 & 2\lambda^2 - 4\lambda + 2
\end{pmatrix}.
\]

999.
\[
\begin{pmatrix}
\lambda & 1 & 1 & \ldots & 1 \\
0 & \lambda & 1 & \ldots & 1 \\
0 & 0 & \lambda & \ldots & 1 \\
\ldots & \ldots & \ldots & \ldots & \ldots \\
0 & 0 & 0 & \ldots & \lambda
\end{pmatrix}.
\]
Выяснить, эквивалентны ли между собой матрицы:
1000.

\[
A = \begin{pmatrix}
3\lambda + 1 & \lambda & 4\lambda - 1 \\
1 - \lambda^2 & \lambda - 1 & \lambda - \lambda^2 \\
\lambda^2 + \lambda + 2 & \lambda & \lambda^2 + 2\lambda
\end{pmatrix};
\]
\[
B = \begin{pmatrix}
\lambda + 1 & \lambda - 2 & \lambda^2 - 2\lambda \\
2\lambda & 2\lambda - 3 & \lambda^2 - 2\lambda \\
-2 & 1 & 1
\end{pmatrix}.
\]

1001.

\[
A = \begin{pmatrix}
\lambda^2 + \lambda + 1 & 3\lambda - \lambda^2 & 2\lambda^2 + \lambda & \lambda^2 \\
\lambda^2 + \lambda & 3\lambda - \lambda^2 & 2\lambda^2 + \lambda & \lambda^2 \\
\lambda^2 - \lambda & 2\lambda - \lambda^2 & 2\lambda^2 + \lambda & \lambda^2 \\
\lambda^2 & -\lambda^2 & 2\lambda^2 & \lambda^2
\end{pmatrix};
\]
\[
B = \begin{pmatrix}
3 & \lambda^2 + 1 & 3\lambda^2 & \lambda^2 \\
2 & \lambda^2 + 1 & 3\lambda^2 & \lambda^2 \\
0 & \lambda^2 & 3\lambda^2 & \lambda^2 \\
\lambda^2 & -\lambda^2 & 2\lambda^2 & \lambda^2
\end{pmatrix}.
\]

1002.

\[
A = \begin{pmatrix}
3\lambda^3 - 6\lambda^2 + \lambda + 3 & 2\lambda^3 - 4\lambda^2 + 3\lambda - 1 & \lambda^3 - 2\lambda^2 + \lambda \\
3\lambda^2 - 8\lambda + 5 & 2\lambda^2 - 4\lambda + 1 & \lambda^2 - 2\lambda + 1 \\
3\lambda^3 - 3\lambda^2 - 5\lambda + 6 & 2\lambda^3 - 2\lambda^2 - \lambda + 1 & \lambda^3 - \lambda^2 - \lambda + 1
\end{pmatrix};
\]
\[
B = \begin{pmatrix}
3\lambda^3 - 9\lambda^2 + 7\lambda + 1 & 2\lambda^3 - 6\lambda^2 + 7\lambda - 2 & \lambda^3 - 3\lambda^2 + 3\lambda - 1 \\
3\lambda^3 - 9\lambda^2 + 9\lambda - 5 & 2\lambda^3 - 6\lambda^2 + 6\lambda - 1 & \lambda^3 - 3\lambda^2 + 3\lambda - 1 \\
3\lambda^3 - 9\lambda^2 + 5\lambda + 5 & 2\lambda^3 - 6\lambda^2 + 8\lambda - 2 & \lambda^3 - 3\lambda^2 + 3\lambda - 1
\end{pmatrix};
\]
\[
C = \begin{pmatrix}
3\lambda^2 - 3\lambda + 1 & \lambda^2 - \lambda & 0 \\
2\lambda^2 - \lambda - 1 & 7\lambda - 3\lambda^2 - 4 & \lambda^2 - 2\lambda + 1 \\
5\lambda^2 - 7\lambda + 3 & 5\lambda - 2\lambda^2 - 3 & \lambda^2 - 2\lambda + 1
\end{pmatrix}.
\]